drastic simplifications CPS event semantics 1) no enque event 2) eMesg returns a single message
 Got bogged down by the complexity. A source of it was having eMesg return
 a list of messages. Perhaps this was designed to avoid have multiple send
 events corresponding to a deq event. At that time, the need of sending
 delayed messages was not anticipated. Now since we have that, sending a
 list directly is almost useless. If the recepient is the same node/topic,
 just augment the topicType to be a pair/list. If the recepients are
 different, the hardware does not send the messages at once anyways.
 Removed enqEvent. Till ITP, wont be able to deal with anyways.

wont fix train for now.

ROSCyberPhysicalSystem.v
@@ -24,8 +24,7 @@ Record SendEvtInfo := mkSendEvtInfo  {
  *)
 Inductive EventKind : Set := 
   | sendEvt (inf : SendEvtInfo) 
-  | enqEvt 
-  | deqEvt (enqIndex: nat).
+  | deqEvt.
 
 
 Section Event.
@@ -41,14 +40,9 @@ Class EventType (T: Type)
     	(minGap : Q) 
       {tdeq: DecEq T}  := {
   eLoc : T ->  Loc;
-  eMesg : T -> list Message;
+  eMesg : T -> Message;
   eKind : T -> EventKind;
   
-  enQDeq1Mesg : forall t, match eKind t with
-                          | enqEvt => length (eMesg t) = 1%nat
-                          | deqEvt _ => length (eMesg t) = 1%nat
-                          | sendEvt _ => True
-                          end;
 
   eTime : T -> QTime;
   timeDistinct : forall (a b : T), 
@@ -209,7 +203,7 @@ Definition isSendEvtOp (ev: option Event) : bool :=
 
 Definition isDeqEvt (ev: Event) : bool :=
   match (eKind ev) with
-  | deqEvt _ => true
+  | deqEvt => true
   | _ => false
   end.
 
@@ -217,18 +211,14 @@ Definition isDeqEvt (ev: Event) : bool :=
 Definition isDeqEvtOp (ev: option Event) : bool :=
   opApPure isDeqEvt false ev.
 
-Definition isEnqEvt (ev: Event) :Prop :=
-eKind ev = enqEvt.
 
-Definition isEnqEvtOp (ev: option Event) :Prop :=
-  opApPure isEnqEvt False ev.
 
 (** !!FIX!! this should be [isEnqEvt] *)
 Definition isRecvEvt := isDeqEvt.
 
 Close Scope Q_scope.
 
-(** FIFO queue axiomatization *)
+(** FIFO queue axiomatization 
 Fixpoint CorrectFIFOQueueUpto   (upto : nat)
     (locEvts: nat -> option Event) :  Prop * list Message :=
 match upto with
@@ -255,24 +245,22 @@ end.
 Definition CorrectFIFOQueue    :  Prop :=
 forall (l: LocT)
  (upto : nat), fst (CorrectFIFOQueueUpto upto (localEvts l)).
+*)
 
-Definition deqMesg (ev : Event) : option Message :=
+Definition deqMesg (ev : Event): option Message :=
 match eKind ev with
- | deqEvt _ => head (eMesg ev)
+ | deqEvt => Some (eMesg ev)
 (** BTW, [(eMesg ev)] is supposed to be a singletop *)
  | _ => None
 end.
 
 Lemma deqSingleMessage : forall evD,
   isDeqEvt evD
-  -> {m : Message | m::nil = eMesg evD /\ (deqMesg evD = Some m)}.
+  -> {m : Message |  m = eMesg evD ∧ (deqMesg evD = Some m)}.
 Proof.
   intros ? Hd.
-  pose proof (enQDeq1Mesg evD) as XX.
   unfold isDeqEvt in Hd.
   unfold deqMesg. destruct (eKind evD); try (inversion Hd; fail);[].
-  destruct ((eMesg evD)); inversion XX.
-  destruct l; inversion H0.
   eexists; eauto.
 Defined.
 
@@ -289,31 +277,22 @@ Qed.
 
 Lemma deqSingleMessage2 : forall evD m,
   Some m = deqMesg evD
-  -> m::nil = eMesg evD.
+  -> m = eMesg evD.
 Proof.
-  intros ? ? Hd. pose proof Hd as Hdb.
-  apply deqMesgSome in Hd.
-  apply deqSingleMessage in Hd.
-  destruct Hd as [m' Hd].
-  repnd.
-  congruence.
+  intros ? ? Hd. unfold deqMesg in Hd.
+  destruct (eKind evD); inversion Hd.
+  reflexivity.
 Defined.
 
-Definition enqMesg (ev : Event) : option Message :=
-match eKind ev with
-| enqEvt => head (eMesg ev)
-| _ => None
-end.
 
-Definition sentMesg (ev : Event) : list Message :=
+Definition sentMesg (ev : Event) : option Message :=
 match eKind ev with
-| sendEvt _ =>  (eMesg ev)
-| _ => nil
+| sendEvt _ =>  Some (eMesg ev)
+| _ => None
 end.
 
 (* these notations have to be defined again at the end of the section *)
 Definition deqMesgOp := (opBind deqMesg).
-Definition enqMesgOp := (opBind enqMesg).
 (* Definition sentMesgOp := (opBind sentMesg). *)
 
 
@@ -329,22 +308,6 @@ Proof.
 Qed.
 
 
-
-
-
-Lemma evEnqHead : forall ev m, 
-    enqEvt = eKind ev
-    -> In m (eMesg ev)
-    -> Some m = head (eMesg ev).
-Proof.
-  intros ? ? Heq Hin.
-  pose proof (enQDeq1Mesg ev) as XX.
-  rewrite <- Heq in XX.
-  eapply length1In in XX; eauto.
-  rewrite <- XX.
-  simpl.
-  reflexivity.
-Qed.
 
 Definition getRecdPayload (tp : RosTopic) (ev : Event) 
   : option (topicType tp)  :=
@@ -378,7 +341,7 @@ Qed.
 
 Lemma getRecdPayloadSpecMesg: forall tp ev tv,
       getRecdPayload tp ev = Some tv
-      -> isDeqEvt ev ∧ map fst (eMesg ev) = (mkMesg tp tv)::nil.
+      -> isDeqEvt ev ∧ π₁ (eMesg ev) = (mkMesg tp tv).
 Proof.
   unfold getRecdPayload. intros ? ? ? Heq.
   pose proof (deqMesgSome ev) as Hd.
@@ -391,7 +354,7 @@ Proof.
   repnd.
   rewrite Hdr in Heqdm.
   inverts Heqdm.
-  apply MsgEta in Heq.
+  apply MsgEta in Heq. 
   rewrite <- Hdl.
   simpl. rewrite Heq.
   reflexivity.
@@ -408,11 +371,11 @@ Proof.
   reflexivity.
 Qed.
 
-Lemma isDeqEvtIf : ∀ {ed enqIndex}, 
-    eKind ed = deqEvt enqIndex
+Lemma isDeqEvtIf : ∀ {ed}, 
+    eKind ed = deqEvt
     -> isDeqEvt ed.
 Proof.
-  intros ? ? Heq.
+  intros ? Heq.
   unfold isDeqEvt.
   destruct  (eKind ed); inversion Heq.
   reflexivity.
@@ -694,6 +657,7 @@ Proof.
 Close Scope Q_scope.
 
 
+(*
 Lemma queueContents : forall  (locEvts: nat -> option Event)
      (upto : nat),
    let (prp, queue) := CorrectFIFOQueueUpto upto locEvts  in
@@ -781,6 +745,7 @@ Proof.
   destruct l1; inversion H1.
   simpl in Heqm. inversion Heqm. reflexivity.
 Qed.
+*)
 
 
 (** first event is innermost, last event is outermost.
@@ -791,7 +756,7 @@ Fixpoint prevProcessedEvents (m : nat)
   | 0 => nil
   | S m' => (match locEvents m' with
               | Some ev => match (eKind ev) with
-                            | deqEvt _ => (ev)::nil
+                            | deqEvt => (ev)::nil
                             | _ => nil
                             end
               | None => nil (* this will never happen *)
@@ -805,6 +770,9 @@ Definition getDeqOutput (proc: Process Message (list Message))
 
 Close Scope Q_scope.
 
+Require Export Coq.Program.Basics.
+
+Open Scope program_scope.
   
 (** assuming all outgoing messages resulting from processing
     an event happen in a single send event (send once) *)
@@ -815,23 +783,20 @@ Definition possibleDeqSendOncePair
   match (locEvts nd, locEvts ns) with
   | (Some evd, Some evs) => 
     isDeqEvt evd ∧ isSendEvt evs ∧ nd < ns (** the last bit is redundant because of time *)
-    ∧ (forall n: nat, nd < n < ns -> isEnqEvtOp (locEvts n))
     ∧ (eTime evd < eTime evs < (eTime evd) + (procTime swNode))%Q
     ∧ let procEvts := prevProcessedEvents nd locEvts in
-      let procMsgs := flat_map eMesg procEvts in
+      let procMsgs := map eMesg procEvts in
       let lastProc := getNewProcL (process swNode) procMsgs in
-      (getDeqOutput lastProc (locEvts nd)) = opBind2 eMesg (locEvts ns)
+      (getDeqOutput lastProc (locEvts nd)) 
+        = opBind2 ((λ m, m::nil)∘ eMesg) (locEvts ns)
   
   | _ => False
   end.
 
 Definition getDeqOutput2 (proc: Process Message (list Message))
   (ev : Event) : (list Message) :=
-   flat_map (getOutput proc) (eMesg ev).
+    (getOutput proc) (eMesg ev).
 
-Require Export Coq.Program.Basics.
-
-Open Scope program_scope.
 
 Definition minDelayForIndex (lm : list Message) (index : nat) : Q :=
   let delays := map (delay ∘ (π₂)) (firstn index lm) in
@@ -842,7 +807,7 @@ Definition procOutMsgs
   (locEvts: nat -> option Event)
   (nd : nat) : list Message := 
     let procEvts := prevProcessedEvents nd locEvts in
-    let procMsgs := flat_map eMesg procEvts in
+    let procMsgs := map eMesg procEvts in
     let lastProc := getNewProcL (process swNode) procMsgs in
     match (locEvts nd) with
     | Some evd => (getDeqOutput2 lastProc evd)
@@ -862,13 +827,12 @@ Definition possibleDeqSendOncePair2
   match (locEvts nd, locEvts ns) with
   | (Some evd, Some evs) =>
       match (eKind evd, eKind evs) with
-      | (deqEvt enqIndex , sendEvt sinf) =>
+      | (deqEvt, sendEvt sinf) =>
             let minDelay := (minDelayForIndex procOutMsgs (startIndex sinf)) in
               ns = (S nd) + sindex
               ∧ sindex = (startIndex sinf)
-              ∧ isPrefixOf (eMesg evs) (skipn sindex procOutMsgs)
+              ∧ Some (eMesg evs) = (nth_error procOutMsgs sindex)
               ∧ ball timingAcc (eTime evd + minDelay + procTime)%Q (QT2Q (eTime evs))
-              ∧ length (eMesg evs) =1
       | (_,_) => False
       end
   | _ => False
@@ -1017,7 +981,7 @@ Definition AllNodeBehCorrect : Type:=
 
 Definition PossibleSendRecvPair
   (Es  Er : Event) : Prop :=
-   (map fst (eMesg Es) = map fst (eMesg Er))
+   (fst (eMesg Es) = fst (eMesg Er))
    /\ (validRecvMesg (validTopics (eLoc Er)) (eMesg Er))
    /\ (validSendMesg (validTopics (eLoc Es)) (eMesg Es))
    /\ (match (maxDeliveryDelay  (eLoc Es) (eLoc Er)) with
@@ -1054,7 +1018,6 @@ Record PossibleEventOrder  := {
                   PossibleSendRecvPair Es Er
                   /\ causedBy Es Er /\ isSendEvt Es};
 
-    corrFIFO : CorrectFIFOQueue;
     corrNodes : AllNodeBehCorrect;
 
 
@@ -1082,13 +1045,12 @@ Lemma PureProcDeqSendOncePair : forall ns nd TI TO qt qac loc
   possibleDeqSendOncePair (Build_RosSwNode sproc (qt,qac)) (localEvts loc) nd ns
   -> {es : Event | {ed : Event | isDeqEvt ed × isSendEvt es
           × (nd < ns)
-            × (∀ n : nat, (nd < n) ∧ (n < ns) → isEnqEvtOp (localEvts loc n))
               × (eTime ed <eTime es < eTime ed + qt)%Q
         × localEvts loc nd = Some ed × localEvts loc ns = Some es ×
           (validRecvMesg (TI::nil,nil) (eMesg ed)
            ->  {dmp : topicType TI |  
-                      map fst (eMesg ed) = ((mkMesg _ dmp)::nil)
-                      ∧ (mkImmMesg TO (sp dmp) )::nil = (eMesg es)})}}.
+                      fst (eMesg ed) = ((mkMesg _ dmp))
+                      ∧ (mkImmMesg TO (sp dmp) ) = (eMesg es)})}}.
 Proof.
   intros ? ? ? ? ? ? ? ?. simpl. intro Hnc.
   unfold possibleDeqSendOncePair in Hnc.
@@ -1104,11 +1066,10 @@ Proof.
   split; [trivial |].
   split; [trivial |].
   split; [trivial |].
-  split; [trivial |].
   split; [reflexivity |].
   split; [reflexivity |].
-  clear Hncrrrl Hncrrl Hncrl Hncl.
-  rename Hncrrrr into Hnc.
+  clear  Hncrrl Hncrl Hncl.
+  rename Hncrrr into Hnc.
   unfold validRecvMesg. simpl.
   intro Hsub.
   apply deqSingleMessage in Hdeq.
@@ -1116,7 +1077,6 @@ Proof.
   clear HeqoevS.
   destruct Hdeq as [dm Hdeq]. repnd.
   rewrite <- Hdeql in Hsub.
-  specialize (Hsub _ (or_introl  eq_refl)).
   rewrite RemoveOrFalse in Hsub.
   symmetry in Hsub.
   exists (transport Hsub (mPayload dm)).
@@ -1126,14 +1086,18 @@ Proof.
   rewrite getNewProcLPure in Hnc.
   rewrite <- Hdeql.
   clear Hdeql Hdeqr. 
-  simpl. inversion Hnc as [Hncc]. clear Hnc Hncc.
-  unfold liftToMesg. unfold getPayload.
+  simpl. inverts Hnc as Hnc. 
+  unfold liftToMesg in Hnc. unfold getPayload in Hnc.
   destruct dm as [dm hdr].
   destruct dm as [dmt dmp].
-  simpl in Hsub.  destruct Hsub.
-  simpl. unfold mtopic. simpl. split;[reflexivity|].
+  simpl in Hnc, Hsub.
+  destruct Hsub.
+  simpl. simpl in Hnc. 
+  unfold mtopic. unfold mtopic in Hnc. simpl. 
+  simpl in Hnc. split;[reflexivity|].
   destruct (eqdec dmt dmt) as [Heq| Hneq];
     [| apply False_rect; apply Hneq; reflexivity].
+  inversion Hnc.
   simpl.
   pose proof (@UIPReflDeq RosTopic _ _ Heq) as Heqr.
   rewrite Heqr.
